\documentclass{article}
\usepackage{ifthen}
\usepackage{epsfig}
\usepackage[utf8]{inputenc}
\usepackage{newunicodechar}
  \newunicodechar{⁻}{${}^{-}$}% Superscript minus
  \newunicodechar{²}{${}^{2}$}% Superscript two
  \newunicodechar{³}{${}^{3}$}% Superscript three

\pagestyle{empty}
\begin{document}
$\forall i,\;f + a_i$
\pagebreak

$\forall i,\;f - a_i$
\pagebreak

$\forall i,\;f\,a_i$
\pagebreak

$\forall i,\;f\;/\;a_i$
\pagebreak

$\infty$
\pagebreak

$a_i=0$
\pagebreak

$\forall i,\;\ln (a_i)$
\pagebreak

$-\infty$
\pagebreak

$a_i\leq 0$
\pagebreak

$\forall i,\;e^{a_i}$
\pagebreak

$v_i$
\pagebreak

$\forall i,\;+t_i$
\pagebreak

$\forall i,\;-t_i$
\pagebreak

$\forall i,\;t_i \rightarrow t_i + a_i$
\pagebreak

$\forall i,\;t_i \rightarrow t_i - a_i$
\pagebreak

$\forall i,\;t_i \rightarrow t_i\,a_i$
\pagebreak

$\forall i,\;t_i \rightarrow t_i\;/\;a_i$
\pagebreak

$t_i \rightarrow \infty$
\pagebreak

$\forall i,\;t_i \rightarrow t_i\;+\;a_i$
\pagebreak

$\forall i,\;t_i \rightarrow t_i\;-\;a_i$
\pagebreak

$\forall i,\;t_i \rightarrow t_i\;a_i$
\pagebreak

$\forall i,\;t_i \rightarrow t_i + f$
\pagebreak

$\forall i,\;t_i \rightarrow t_i - f$
\pagebreak

$\forall i,\;t_i \rightarrow t_i\,f$
\pagebreak

$\forall i,\;t_i \rightarrow t_i\;/\;f$
\pagebreak

$f=0$
\pagebreak

$\forall i, t_i + f$
\pagebreak

$\forall i,\; t_i - f$
\pagebreak

$\forall i,\; t_i\,f$
\pagebreak

$\forall i,\; t_i\;/\;f$
\pagebreak

$\frac{1}{3}$
\pagebreak

$\pi$
\pagebreak

$2\pi$
\pagebreak

$4\pi$
\pagebreak

$\frac{4\pi}{3}$
\pagebreak

$n_e-n_p\sum_{i=1}^{nms}f_i\;\bar{z}_i(T_e,T_r,n_e)$
\pagebreak

$x_i$
\pagebreak

$y_i$
\pagebreak

$w_i$
\pagebreak

$weight \times \sum_{i=0}^{n-1} | w_i (a_i - y_i) |$
\pagebreak

$weight \times \sum_{i=0}^{n-1} w_i (a_i - y_i)^2$
\pagebreak

$-\chi^2$
\pagebreak

$1 \leq i \leq n$
\pagebreak

$1 \leq j \leq freq$
\pagebreak

$j=freq,\;j\rightarrow 0$
\pagebreak

$ax^2+bx+c=0$
\pagebreak

$a=0$
\pagebreak

$b=0$
\pagebreak

$n_e = n_p \sum_{i=1}^{nmat} f_{pi}\;\bar{z_i}$
\pagebreak

$ tev \leq 0 $
\pagebreak

$\frac{1}{\sigma\sqrt{2\pi}}\;e^{-\frac{(x-\mu)^2}{2\sigma^2}}$
\pagebreak

$y=f(x)$
\pagebreak

$\int_a^b f(x)\;dx$
\pagebreak

$(f*g)(x)=\int_{-\infty}^\infty\;f(t)\;g(x-t)\;dt$
\pagebreak

$f\;\vec{t}$
\pagebreak

$ v = |\vec{v}| $
\pagebreak

$ |\vec{t}-\vec{v}| $
\pagebreak

$+\vec{v}$
\pagebreak

$-\vec{v}$
\pagebreak

$\vec{t}\rightarrow\vec{t}+\vec{v}$
\pagebreak

$\vec{t}\rightarrow\vec{t}-\vec{v}$
\pagebreak

$\vec{t}+\vec{v}$
\pagebreak

$\vec{t}-\vec{v}$
\pagebreak

$\vec{t}\rightarrow\vec{t}\;g$
\pagebreak

$\vec{t}\rightarrow\vec{t}\;/\;g$
\pagebreak

$g=0$
\pagebreak

$\vec{t}\;f$
\pagebreak

$\vec{t}\;/\;g$
\pagebreak

$\hat{t}=\vec{t}/t$
\pagebreak

$\vec{t}\rightarrow -\vec{t}$
\pagebreak

$\vec{t}\bullet\vec{v}$
\pagebreak

$\vec{t}\rightarrow\vec{t}\times\vec{v}$
\pagebreak

$\vec{t}\times\vec{v}$
\pagebreak

$\hat{t}\bullet\hat{v}$
\pagebreak

$\arccos ( \hat{t}\bullet\hat{v} )$
\pagebreak

$\vec{t}$
\pagebreak

$\vec{v_{\parallel}}=(\vec{t}\bullet\hat{v})\;\hat{v}$
\pagebreak

$\vec{v_{\perp}}=\vec{t}-\vec{v_{\parallel}}$
\pagebreak

$(\sqrt{x^2+y^2}\;,z\;,0)$
\pagebreak

\end{document}
